feat(USubst): Efficient One-pass

DLean/USubst/Subst.lean
@@ -253,6 +253,20 @@ next hin =>
 
 end
 
+/- Precomputes the bound variables post-substitution.
+   Used for substitution of loops. -/
+def Program.substBoundVars (σ : Subst) (α : Program) : FCSet Assignable :=
+  match α with
+  | .const a => (σ.get a).boundVars'
+  | .test _ => ∅
+  | .assign x _
+  | .random x => {x}
+  | .choice α β
+  | .seq α β => α.substBoundVars σ ∪ β.substBoundVars σ
+  | .loop α => α.substBoundVars σ
+  | .ode _ _ => α.boundVars'
+
+
 mutual
 
 def Formula.applySubst (σ : Subst) (U : FCSet Assignable) (Φ : Formula) : Option Formula := match Φ with
@@ -267,15 +281,13 @@ def Formula.applySubst (σ : Subst) (U : FCSet Assignable) (Φ : Formula) : Opti
   | .exists x Φ       => do
       return .exists x (← Φ.applySubst σ ({.var x} ∪ U))
   | .diamond α Φ      => do
-      let σα ← α.applySubst σ U
-      let V := σα.boundVars' ∪ U
+      let ⟨V,σα⟩ ← α.applySubst σ U
       return .diamond σα (← Φ.applySubst σ V)
   | .box α Φ          => do
-      let σα ← α.applySubst σ U
-      let V := σα.boundVars' ∪ U
+      let ⟨V,σα⟩ ← α.applySubst σ U
       return .box σα (← Φ.applySubst σ V)
   | .ref α β          => do
-      return .ref (← α.applySubst σ U) (← β.applySubst σ U)
+      return .ref (← α.applySubst σ U).2 (← β.applySubst σ U).2
   | .applyPred p args => do
       let sargs ← TermVector.applySubst σ U args
       if (.Predicate p) ∈ σ then
@@ -291,29 +303,33 @@ next hin =>
   apply Subst.symbol_size at hin
   grind only [= Prod.lex_def]
 
-def Program.applySubst (σ : Subst) (U : FCSet Assignable) (α : Program) : Option Program := match α with
-  | .assign x t   => return .assign x (← t.applySubst σ U)
-  | .random x     => return .random x
-  | .test Φ       => return .test (← Φ.applySubst σ U)
+def Program.applySubst (σ : Subst) (U : FCSet Assignable) (α : Program) : Option (FCSet Assignable × Program) := match α with
+  | .assign x t   => return ⟨{x} ∪ U, .assign x (← t.applySubst σ U)⟩
+  | .random x     => return ⟨{x} ∪ U, .random x⟩
+  | .test Φ       => return ⟨U, .test (← Φ.applySubst σ U)⟩
   | .ode system Ψ => do
-    let vars := (system.map ODE.var).toFinset
+    let vars := system.assignables
     let vars' := vars.map Assignable.diff_emb
     let V := (.Finite (vars ∪ vars')) ∪ U
     let σΨ ← Ψ.applySubst σ V
 
     let ssystem ← system.mapM (fun {var, term} => do return ODE.mk var (← Term.applySubst σ V term))
-    return .ode ssystem σΨ
-  | .choice α β   => return .choice (← α.applySubst σ U) (← β.applySubst σ U)
+    return ⟨V, .ode ssystem σΨ⟩
+  | .choice α β   => do
+    let ⟨V, σα⟩ ← α.applySubst σ U
+    let ⟨W, σβ⟩ ← β.applySubst σ U
+    return ⟨V ∪ W, .choice σα σβ⟩
   | .seq α β      => do
-    let σα ← α.applySubst σ U
-    let V := σα.boundVars' ∪ U
-    return .seq σα (← β.applySubst σ V)
+    let ⟨V, σα⟩ ← α.applySubst σ U
+    let ⟨W, σβ⟩ ← β.applySubst σ V
+    return ⟨W, .seq σα σβ⟩
   | .loop α       => do
-    let σα ← α.applySubst σ U
-    let V := σα.boundVars' ∪ U
-    let σα' ← α.applySubst σ V
-    return .loop σα'
-  | .const a      => return Subst.get σ a
+    let V := α.substBoundVars σ ∪ U
+    let ⟨W,σα⟩ ← α.applySubst σ V
+    return ⟨W, .loop σα⟩
+  | .const a      =>
+    let σα := Subst.get σ a
+    return ⟨σα.boundVars' ∪ U, σα⟩
 termination_by (σ.size, α.size)
 decreasing_by
 all_goals (simp_all[Program.size] ; grind)
@@ -877,11 +893,74 @@ decreasing_by
 
 end
 
-/- Proof that applySubst's output does not on the taboo, as long as it does not clash. -/
+/- Substitution preserves ode's assignables -/
+lemma ode_mapM_assignables_eq
+  {σ : Subst}
+  {U : FCSet Assignable}
+  {system : OdeSystem}
+  {ssystem : OdeSystem}
+  (h : system.mapM (fun x => do return ODE.mk x.var (← Term.applySubst σ U x.term))
+       = some ssystem)
+  : OdeSystem.assignables ssystem = OdeSystem.assignables system := by
+  unfold OdeSystem.assignables at *;
+  induction system generalizing ssystem <;> simp_all +decide [ List.mapM_cons ];
+  cases h' : Term.applySubst σ U ‹ODE›.term <;> simp_all +decide [ Option.bind_eq_some_iff ];
+  aesop
+
+/- `Program.substBoundVars` computes the bound variables of the substituted program -/
+lemma Program.substBoundVars_applySubst_boundVars
+  (σ : Subst)
+  (U V : FCSet Assignable)
+  (α α' : Program) :
+  Program.applySubst σ U α = some ⟨V,α'⟩ → α'.boundVars' = α.substBoundVars σ := by
+  intro h
+  match α with
+  | .const _
+  | .test _
+  | .assign _ _
+  | .random _ =>
+    simp[Program.applySubst, Option.bind] at h
+    grind only [substBoundVars, boundVars']
+  | .choice β γ
+  | .seq β γ =>
+    simp[Program.applySubst, Option.bind] at h
+    split at h
+    . contradiction
+    simp only at h
+    split at h
+    . contradiction
+    simp at h
+    next β' hβ _ _ γ' hγ =>
+      apply Program.substBoundVars_applySubst_boundVars at hγ
+      apply Program.substBoundVars_applySubst_boundVars at hβ
+      grind only [substBoundVars, boundVars', = Set.subset_def, = Set.mem_union]
+  | .loop β =>
+    simp[Program.applySubst, Option.bind] at h
+    split at h
+    . contradiction
+    simp at h
+    next β' hβ =>
+      apply Program.substBoundVars_applySubst_boundVars at hβ
+      grind only [substBoundVars, boundVars', = Set.subset_def, = Set.mem_union]
+  | .ode sys _ =>
+    simp[Program.applySubst, Option.bind] at h
+    split at h
+    . contradiction
+    simp only at h
+    split at h
+    . contradiction
+    simp at h
+    next sys' hsys =>
+      have hassign : OdeSystem.assignables sys' = OdeSystem.assignables sys :=
+          ode_mapM_assignables_eq (show _ = some sys' from ‹_›)
+      grind only [substBoundVars, boundVars', FCSet.to_set_eq, = Set.subset_def, = Set.mem_union, = Finset.mem_coe,
+        = Set.mem_image, = Finset.mem_map]
+
+/- Weakening the taboo does not create clash. -/
 mutual
 
-lemma TermVector.applySubst_unique {σ : Subst} {U V : FCSet Assignable} {n : ℕ} {ts ts₁ ts₂ : TermVector n} :
-  ts.applySubst σ U = ts₁ → ts.applySubst σ V = ts₂ → ts₁ = ts₂ := by
+lemma TermVector.taboo_mono {σ : Subst} {U V : FCSet Assignable} {n : ℕ} {ts ts' : TermVector n} :
+  V.toSet ⊆ U.toSet → ts.applySubst σ U = ts' → ts.applySubst σ V = ts' := by
   match n with
   | 0 => match ts with
     | .nil =>
@@ -889,13 +968,13 @@ lemma TermVector.applySubst_unique {σ : Subst} {U V : FCSet Assignable} {n : �
   | n+1 => match ts with
     | .cons t ts' =>
       simp_all[TermVector.applySubst, Option.bind_eq_some_iff]
-      intro _ h₁ _ h₁' _ _ h₂ _ h₂'
-      have := Term.applySubst_unique h₁ h₂
-      have := TermVector.applySubst_unique h₁' h₂'
+      intro hUV _ h₁ _ h₂
+      have := Term.taboo_mono hUV h₁
+      have := TermVector.taboo_mono hUV h₂
       grind only
 
-lemma Term.applySubst_unique {σ : Subst} {U V : FCSet Assignable} {t t₁ t₂ : Term} :
-  t.applySubst σ U = t₁ → t.applySubst σ V = t₂ → t₁ = t₂ := by
+lemma Term.taboo_mono {σ : Subst} {U V : FCSet Assignable} {t t' : Term} :
+  V.toSet ⊆ U.toSet → t.applySubst σ U = t' → t.applySubst σ V = t' := by
   match t with
   | .var _
   | .applyFn (Fn.num _) _
@@ -903,48 +982,50 @@ lemma Term.applySubst_unique {σ : Subst} {U V : FCSet Assignable} {t t₁ t₂ 
     grind only [Term.applySubst]
   | .neg _ =>
     simp[Term.applySubst, Option.bind_eq_some_iff]
-    intro _ h₁ _ _ h₂
-    have := Term.applySubst_unique h₁ h₂
+    intro hUV _ h
+    have := Term.taboo_mono hUV h
     grind only
   | .plus _ _
   | .times _ _ =>
     simp[Term.applySubst, Option.bind_eq_some_iff]
-    intro _ h₁ _ h₁' _ _ h₂ _ h₂'
-    have := Term.applySubst_unique h₁ h₂
-    have := Term.applySubst_unique h₁' h₂'
+    intro hUV _ h₁ _ h₂
+    have := Term.taboo_mono hUV h₁
+    have := Term.taboo_mono hUV h₂
     grind only
   | .applyFn (Fn.sym _) _ =>
     simp[Term.applySubst, Option.bind_eq_some_iff]
-    intro _ hθ₁ h₁ _ hθ₂ h₂
-    have := TermVector.applySubst_unique hθ₁ hθ₂
-    rw[this] at h₁
-    split at h₁
+    intro hUV _ h₁ h₂
+    apply TermVector.taboo_mono hUV at h₁
+    split at h₂
     . simp_all[Option.bind]
-      split at h₁
-      . contradiction
       split at h₂
       . contradiction
       simp_all
+      suffices (↑(Term.freeVars (σ.get (Symbol.Function _))) ∩ V.toSet = ∅) by
+        rw[this]
+        simp
+      grind only [= Set.subset_def, = Set.mem_inter_iff, = Set.mem_empty_iff_false]
     . simp_all
 end
 
-lemma ode_mapM_applySubst_unique {σ : Subst} {U V : FCSet Assignable} {sys sys₁ sys₂ : OdeSystem} :
-  sys.mapM (fun x => do return ODE.mk x.var (← Term.applySubst σ U x.term)) = some sys₁ →
-  sys.mapM (fun x => do return ODE.mk x.var (← Term.applySubst σ V x.term)) = some sys₂ →
-  sys₁ = sys₂ := by
+lemma ode_mapM_taboo_mono {σ : Subst} {U V : FCSet Assignable} {sys sys' : OdeSystem} :
+  V.toSet ⊆ U.toSet →
+  sys.mapM (fun x => do return ODE.mk x.var (← Term.applySubst σ U x.term)) = some sys' →
+  sys.mapM (fun x => do return ODE.mk x.var (← Term.applySubst σ V x.term)) = some sys' := by
   match sys with
   | .nil =>
     simp_all
   | .cons _ _ =>
     simp_all[Option.bind_eq_some_iff]
-    intro _ h₁ _ h₁' _ _ h₂ _ h₂'
-    have := Term.applySubst_unique h₁ h₂
-    have := ode_mapM_applySubst_unique h₁' h₂'
-    grind only
+    intro hUV _ h₁ _ h₂
+    have := Term.taboo_mono hUV h₁
+    have := ode_mapM_taboo_mono hUV h₂
+    simp_all only [Option.pure_def, Option.bind_eq_bind, Option.some.injEq, exists_eq_left',
+      implies_true]
 
 mutual
-lemma Formula.applySubst_unique {σ : Subst} {U V : FCSet Assignable} {φ ψ₁ ψ₂ : Formula} :
-  φ.applySubst σ U = ψ₁ → φ.applySubst σ V = ψ₂ → ψ₁ = ψ₂ := by
+lemma Formula.taboo_mono {σ : Subst} {U V : FCSet Assignable} {φ ψ : Formula} :
+  V.toSet ⊆ U.toSet → φ.applySubst σ U = ψ → φ.applySubst σ V = ψ := by
   match φ with
   | .True
   | .False =>
@@ -952,83 +1033,171 @@ lemma Formula.applySubst_unique {σ : Subst} {U V : FCSet Assignable} {φ ψ₁ 
   | .gte _ _
   | .eq _ _ =>
     simp[Formula.applySubst, Option.bind_eq_some_iff]
-    intro _ h₁ _ h₁' _ _ h₂ _ h₂'
-    have := Term.applySubst_unique h₁ h₂
-    have := Term.applySubst_unique h₁' h₂'
+    intro hUV _ h₁ _ h₂
+    have := Term.taboo_mono hUV h₁
+    have := Term.taboo_mono hUV h₂
     grind only
-  | .not _
-  | .exists _ _
-  | .forall _ _ =>
+  | .not _ =>
     simp[Formula.applySubst, Option.bind_eq_some_iff]
-    intro _ h₁ _ _ h₂
-    have := Formula.applySubst_unique h₁ h₂
+    intro hUV _ h
+    have := Formula.taboo_mono hUV h
+    grind only
+  | .exists x _
+  | .forall x _ =>
+    simp[Formula.applySubst, Option.bind_eq_some_iff]
+    intro hUV _ h
+    have : ({.var x} ∪ V).toSet ⊆ ({.var x} ∪ U).toSet := by
+      grind only [= Set.subset_def, FCSet.to_set_union, = Set.mem_union]
+    apply Formula.taboo_mono this at h
     grind only
   | .and _ _ =>
     simp[Formula.applySubst, Option.bind_eq_some_iff]
-    intro _ h₁ _ h₁' _ _ h₂ _ h₂'
-    have := Formula.applySubst_unique h₁ h₂
-    have := Formula.applySubst_unique h₁' h₂'
+    intro hUV _ h₁ _ h₂
+    have := Formula.taboo_mono hUV h₁
+    have := Formula.taboo_mono hUV h₂
     grind only
-  | .box _ _
-  | .diamond _ _ =>
+  | .box α _
+  | .diamond α _ =>
     simp[Formula.applySubst, Option.bind_eq_some_iff]
-    intro _ h₁ _ h₁' _ _ h₂ _ h₂'
-    have := Program.applySubst_unique h₁ h₂
-    have := Formula.applySubst_unique h₁' h₂'
-    grind only
+    intro hUV W _ h₁ _ h₂
+    have := Program.taboo_mono hUV h₁
+    have : α.substBoundVars σ ∪ U = W := by
+      have := Program.taboo_mono (Set.Subset.refl _) h₁
+      grind only
+    rw[←this] at h₂
+    have : (α.substBoundVars σ ∪ V).toSet ⊆ (α.substBoundVars σ ∪ U).toSet := by
+      grind only [= Set.subset_def, FCSet.to_set_union, = Set.mem_union]
+    have := Formula.taboo_mono this h₂
+    grind only [FCSet.to_set_union, = Set.mem_union]
   | .ref _ _ =>
     simp[Formula.applySubst, Option.bind_eq_some_iff]
-    intro _ h₁ _ h₁' _ _ h₂ _ h₂'
-    have := Program.applySubst_unique h₁ h₂
-    have := Program.applySubst_unique h₁' h₂'
+    intro hUV _ _ h₁ _ _ h₂
+    have := Program.taboo_mono hUV h₁
+    have := Program.taboo_mono hUV h₂
     grind only
   | .applyPred _ _ =>
     simp[Formula.applySubst, Option.bind_eq_some_iff]
-    intro _ hθ₁ h₁ _ hθ₂ h₂
-    have := TermVector.applySubst_unique hθ₁ hθ₂
-    rw[this] at h₁
-    split at h₁
+    intro hUV _ h₁ h
+    have := TermVector.taboo_mono hUV h₁
+    split at h
     . simp_all[Option.bind]
-      split at h₁
-      . contradiction
-      split at h₂
+      split at h
       . contradiction
       simp_all
+      suffices (↑(Formula.freeVars' (σ.get (Symbol.Predicate _))) ∩ V.toSet = ∅) by
+        rw[this]
+        simp
+      grind only [= Set.subset_def, = Set.mem_inter_iff, = Set.mem_empty_iff_false]
     . simp_all
 
-lemma Program.applySubst_unique {σ : Subst} {U V : FCSet Assignable} {α β₁ β₂ : Program} :
-  α.applySubst σ U = β₁ → α.applySubst σ V = β₂ → β₁ = β₂ := by
+lemma Program.taboo_mono {σ : Subst} {U V W: FCSet Assignable} {α β : Program} :
+  V.toSet ⊆ U.toSet → α.applySubst σ U = some ⟨W, β⟩ → α.applySubst σ V = some ⟨α.substBoundVars σ ∪ V, β⟩ := by
   match α with
   | .const _
   | .random _ =>
-    grind only [Program.applySubst]
+    grind only [Program.applySubst, Program.substBoundVars, = Option.pure_apply]
   | .test _ =>
-    simp[Program.applySubst, Option.bind_eq_some_iff]
-    intro _ h₁ _ _ h₂
-    have := Formula.applySubst_unique h₁ h₂
+    simp[Program.applySubst, Program.substBoundVars, Option.bind_eq_some_iff]
+    intro hUV _ h
+    have := Formula.taboo_mono hUV h
     grind only
   | .assign _ _ =>
-    simp[Program.applySubst, Option.bind_eq_some_iff]
-    intro _ h₁ _ _ h₂
-    have := Term.applySubst_unique h₁ h₂
+    simp[Program.applySubst, Program.substBoundVars, Option.bind_eq_some_iff]
+    intro hUV _ h
+    have := Term.taboo_mono hUV h
     grind only
-  | .seq _ _
   | .choice _ _ =>
-    simp[Program.applySubst, Option.bind_eq_some_iff]
-    intro _ h₁ _ h₁' _ _ h₂ _ h₂'
-    have := Program.applySubst_unique h₁ h₂
-    have := Program.applySubst_unique h₁' h₂'
-    grind only
-  | .loop _ =>
-    simp[Program.applySubst, Option.bind_eq_some_iff]
-    intro _ _ _ h₁' _ _ _ _ h₂'
-    have := Program.applySubst_unique h₁' h₂'
-    grind only
-  | .ode _ _ =>
-    simp[Program.applySubst, Option.bind_eq_some_iff]
-    intro _ h₁ _ h₁' _ _ h₂ _ h₂'
-    have := Formula.applySubst_unique h₁ h₂
-    have := ode_mapM_applySubst_unique h₁' h₂'
-    grind only
+    simp[Program.applySubst, Program.substBoundVars, Option.bind_eq_some_iff]
+    intro hUV _ _ h₁ _ _ h₂
+    have := Program.taboo_mono hUV h₁
+    have := Program.taboo_mono hUV h₂
+    grind only [FCSet.to_set_union, = Set.mem_union]
+  | .seq α _ =>
+    simp[Program.applySubst, Program.substBoundVars, Option.bind_eq_some_iff]
+    intro hUV W _ h₁ _ _ h₂
+    have := Program.taboo_mono hUV h₁
+    have : α.substBoundVars σ ∪ U = W := by
+      have := Program.taboo_mono (Set.Subset.refl _) h₁
+      grind only
+    rw[←this] at h₂
+    have : (α.substBoundVars σ ∪ V).toSet ⊆ (α.substBoundVars σ ∪ U).toSet := by
+      grind only [= Set.subset_def, FCSet.to_set_union, = Set.mem_union]
+    have := Program.taboo_mono this h₂
+    grind only [FCSet.to_set_union, = Set.mem_union]
+  | .loop α =>
+    simp[Program.applySubst, Program.substBoundVars, Option.bind_eq_some_iff]
+    intro hUV _ _ h₁ _ h₂
+    have : (α.substBoundVars σ ∪ V).toSet ⊆ (α.substBoundVars σ ∪ U).toSet := by
+      grind only [= Set.subset_def, FCSet.to_set_union, = Set.mem_union]
+    have := Program.taboo_mono this h₁
+    grind only [FCSet.to_set_union, = Set.mem_union]
+  | .ode sys _ =>
+    simp[Program.applySubst, Program.substBoundVars, Option.bind_eq_some_iff, -FCSet.to_set_eq]
+    intro  hUV _ h₁ _ h₂
+    set BV := FCSet.Finite (sys.assignables ∪ Finset.map Assignable.diff_emb sys.assignables)
+    have hUV' : (BV ∪ V).toSet ⊆ (BV ∪ U).toSet := by
+      grind only [= Set.subset_def, FCSet.to_set_union, = Set.mem_union]
+    have := Formula.taboo_mono hUV' h₁
+    have := ode_mapM_taboo_mono hUV' h₂
+    simp_all[BV, Program.boundVars']
+
 end
+
+/- Corollary: USubst updated taboo coincides with `Program.substBoundVars`. -/
+theorem Program.substBoundVars_applySubst {σ : Subst} {α α' : Program} {U V : FCSet Assignable} :
+  α.applySubst σ U = some ⟨V, α'⟩ → α.substBoundVars σ ∪ U = V := by
+  intro h
+  have := Program.taboo_mono (Set.Subset.refl _) h
+  grind only
+
+/- Corollary: applySubst's output is unique (w.r.t the taboo), as long as it does not clash. -/
+
+lemma TermVector.applySubst_unique {σ : Subst} {U V : FCSet Assignable} {n : ℕ} {ts ts₁ ts₂ : TermVector n} :
+  ts.applySubst σ U = ts₁ → ts.applySubst σ V = ts₂ → ts₁ = ts₂ := by
+  intro h₁ h₂
+  obtain ⟨hU,hV⟩ : (U ∩ V).toSet ⊆ U.toSet ∧ (U ∩ V).toSet ⊆ V.toSet := by
+    grind only [= Set.subset_def, FCSet.to_set_inter, = Set.mem_inter_iff]
+  apply TermVector.taboo_mono hU at h₁
+  apply TermVector.taboo_mono hV at h₂
+  grind only
+
+lemma Term.applySubst_unique {σ : Subst} {U V : FCSet Assignable} {t t₁ t₂ : Term} :
+  t.applySubst σ U = t₁ → t.applySubst σ V = t₂ → t₁ = t₂ := by
+  intro h₁ h₂
+  obtain ⟨hU,hV⟩ : (U ∩ V).toSet ⊆ U.toSet ∧ (U ∩ V).toSet ⊆ V.toSet := by
+    grind only [= Set.subset_def, FCSet.to_set_inter, = Set.mem_inter_iff]
+  apply Term.taboo_mono hU at h₁
+  apply Term.taboo_mono hV at h₂
+  grind only
+
+
+lemma ode_mapM_applySubst_unique {σ : Subst} {U V : FCSet Assignable} {sys sys₁ sys₂ : OdeSystem} :
+  sys.mapM (fun x => do return ODE.mk x.var (← Term.applySubst σ U x.term)) = some sys₁ →
+  sys.mapM (fun x => do return ODE.mk x.var (← Term.applySubst σ V x.term)) = some sys₂ →
+  sys₁ = sys₂ := by
+  intro h₁ h₂
+  obtain ⟨hU,hV⟩ : (U ∩ V).toSet ⊆ U.toSet ∧ (U ∩ V).toSet ⊆ V.toSet := by
+    grind only [= Set.subset_def, FCSet.to_set_inter, = Set.mem_inter_iff]
+  apply ode_mapM_taboo_mono hU at h₁
+  apply ode_mapM_taboo_mono hV at h₂
+  grind only
+
+lemma Formula.applySubst_unique {σ : Subst} {U V : FCSet Assignable} {φ ψ₁ ψ₂ : Formula} :
+  φ.applySubst σ U = ψ₁ → φ.applySubst σ V = ψ₂ → ψ₁ = ψ₂ := by
+  intro h₁ h₂
+  obtain ⟨hU,hV⟩ : (U ∩ V).toSet ⊆ U.toSet ∧ (U ∩ V).toSet ⊆ V.toSet := by
+    grind only [= Set.subset_def, FCSet.to_set_inter, = Set.mem_inter_iff]
+  apply Formula.taboo_mono hU at h₁
+  apply Formula.taboo_mono hV at h₂
+  grind only
+
+lemma Program.applySubst_unique {σ : Subst} {U V W₁ W₂ : FCSet Assignable} {α β₁ β₂ : Program} :
+  α.applySubst σ U = some ⟨W₁, β₁⟩ → α.applySubst σ V = some ⟨W₂, β₂⟩ → β₁ = β₂ := by
+  intro h₁ h₂
+  obtain ⟨hU,hV⟩ : (U ∩ V).toSet ⊆ U.toSet ∧ (U ∩ V).toSet ⊆ V.toSet := by
+    grind only [= Set.subset_def, FCSet.to_set_inter, = Set.mem_inter_iff]
+  apply Program.taboo_mono hU at h₁
+  apply Program.taboo_mono hV at h₂
+  grind only
+
 end Theorems
